theories/L6_PCPS/ctx_approx.v
@@ -4,14 +4,12 @@
 
 Require Import Coq.Arith.Arith Coq.NArith.BinNat Coq.Lists.List Coq.omega.Omega
         Coq.Relations.Relations Coq.Classes.RelationClasses.
-Require Import L6.cps L6.ctx L6.eval L6.logical_relations L6.identifiers.
+From L6 Require Import cps ctx eval logical_relations identifiers tactics.
 
 Import ListNotations.
 
 
 Definition empty_env := M.empty val.
-
-Ltac inv H := inversion H; clear H; subst.
 
 Section ctx_approx.
 
